src/ldrfpf/LocalPF.v
@@ -1243,4 +1243,11 @@ Proof.
     ii. eapply RACEFREE; cycle 2; eauto. etrans; eauto.
   Qed.
 
+  Lemma pf_racy_read_step_step
+        loc to e tid c1 c2
+        (STEP: pf_racy_read_step loc to e tid c1 c2):
+    pf_step e tid c1 c2.
+  Proof.
+    inv STEP. econs; eauto.
+  Qed.
 End LOCALPF.
