src/ldrfra/LocalDRFRA.v
@@ -36,18 +36,18 @@ Require Import PFtoRA.
 Set Implicit Arguments.
 
 
-Theorem local_drf_ra
-        L s
-        (RACEFREE: RARace.racefree_syn L s):
-  behaviors Configuration.step (Configuration.init s) <1=
-  behaviors (@OrdConfiguration.step L Ordering.acqrel) (Configuration.init s).
-Proof.
-  i.
-  specialize (PFtoRA.init_sim_conf L s). intro SIM.
-  specialize (PFtoRA.init_wf_pf L s). intro WF_PF.
-  specialize (PFtoRA.init_wf_j s). intro WF_J.
-  specialize (PFtoRA.init_wf_ra s). intro WF_RA.
-  ii. exploit (@local_DRFPF L); eauto.
-  { eapply PFtoRA.sim_conf_racefree; eauto. }
-  eapply PFtoRA.sim_conf_behavior; eauto.
-Qed.
+(* Theorem local_drf_ra *)
+(*         L s *)
+(*         (RACEFREE: RARace.racefree_syn L s): *)
+(*   behaviors Configuration.step (Configuration.init s) <1= *)
+(*   behaviors (@OrdConfiguration.step L Ordering.acqrel) (Configuration.init s). *)
+(* Proof. *)
+(*   i. *)
+(*   specialize (PFtoRA.init_sim_conf L s). intro SIM. *)
+(*   specialize (PFtoRA.init_wf_pf L s). intro WF_PF. *)
+(*   specialize (PFtoRA.init_wf_j s). intro WF_J. *)
+(*   specialize (PFtoRA.init_wf_ra s). intro WF_RA. *)
+(*   ii. exploit (@local_DRFPF L); eauto. *)
+(*   { eapply PFtoRA.sim_conf_racefree; eauto. } *)
+(*   eapply PFtoRA.sim_conf_behavior; eauto. *)
+(* Qed. *)
